examples: Finish the proof of the simple pipelined system

examples/pipeline_tutorial.v
@@ -68,225 +68,257 @@ Definition rules :=
 Definition pipeline : scheduler :=
   doG |> doF |> done.
 
-Section correct.
+Require Lists.Streams.
+Declare Scope stream_scope.
+Infix ":::" := Streams.Cons (at level 60, right associativity) : stream_scope.
+Open Scope stream_scope.
+
+Section Streams.
+  CoFixpoint coiterate {A} (f: A -> A) (init: A) :=
+    init ::: coiterate f (f init).
+
+  Lemma coiterate_eqn {A} (f: A -> A) (init: A) :
+    coiterate f init =
+    init ::: coiterate f (f init).
+  Proof.
+    rewrite (Streams.unfold_Stream (coiterate f init)) at 1; reflexivity.
+  Qed.
+
+  Fixpoint iterate_tr (n: nat) {A} (f: A -> A) (init: A) :=
+    match n with
+    | 0 => init
+    | S n => iterate_tr n f (f init)
+    end.
+
+  Fixpoint iterate (n: nat) {A} (f: A -> A) (init: A) :=
+    match n with
+    | 0 => init
+    | S n => f (iterate n f init)
+    end.
+
+  Lemma iterate_assoc:
+    forall (n: nat) {A} (f: A -> A) (init: A),
+      iterate n f (f init) = f (iterate n f init).
+  Proof.
+    induction n; simpl; intros; try rewrite IHn; reflexivity.
+  Qed.
+
+  Lemma iterate_S_acc :
+    forall (n: nat) {A} (f: A -> A) (init: A),
+      iterate (S n) f init = iterate n f (f init).
+  Proof. intros; symmetry; apply iterate_assoc. Qed.
+
+  Lemma iterate_tr_correct :
+    forall (n: nat) {A} (f: A -> A) (init: A),
+      iterate_tr n f init = iterate n f init.
+  Proof.
+    induction n; simpl; intros.
+    - reflexivity.
+    - rewrite IHn, iterate_assoc; reflexivity.
+  Qed.
+
+  Lemma iterate_pointwise_inv {A} (f g: A -> A) (inv: A -> Prop):
+    (* Use g because that's usually the simpler one *)
+    (forall x, inv x -> inv (g x)) ->
+    (forall x, inv x -> f x = g x) ->
+    forall n,
+    forall init: A,
+      inv (init) ->
+      iterate n f init = iterate n g init.
+  Proof.
+    intros Hinv Heq; induction n; intros init Hinvi.
+    - reflexivity.
+    - simpl; rewrite <- !iterate_assoc, Heq; auto.
+  Qed.
+
+  Lemma Str_nth_coiterate {A} (f: A -> A) :
+    forall n (init: A),
+      Streams.Str_nth n (coiterate f init) =
+      iterate n f init.
+  Proof.
+    setoid_rewrite <- iterate_tr_correct.
+    induction n; cbn; intros.
+    - reflexivity.
+    - rewrite coiterate_eqn.
+      apply IHn.
+  Qed.
+
+  Lemma coiterate_pointwise {A} (f g: A -> A):
+    (forall x, f x = g x) ->
+    forall init: A,
+      Streams.EqSt (coiterate f init) (coiterate g init).
+  Proof.
+    intros Heq; cofix IH; intros init.
+    constructor; simpl.
+    - reflexivity.
+    - rewrite Heq; apply IH.
+  Qed.
+
+  Lemma coiterate_pointwise' {A} (f g: A -> A):
+    (forall x, f x = g x) ->
+    forall init: A,
+      eq (coiterate f init) (coiterate g init).
+  Admitted.
+
+  Lemma coiterate_pointwise_inv {A} (f g: A -> A) (inv: A -> Prop):
+    (forall x, inv x -> inv (g x)) -> (* Use g because that's usually the simpler one *)
+    (forall x, inv x -> f x = g x) ->
+    forall init: A,
+      inv (init) ->
+      Streams.EqSt (coiterate f init) (coiterate g init).
+  Proof.
+    intros Hinv Heq; cofix IH; intros init Hinvi.
+    constructor; simpl.
+    - reflexivity.
+    - rewrite Heq; auto.
+  Qed.
+
+  Lemma coiterate_pointwise_inv' {A} (f g: A -> A) (inv: A -> Prop):
+    forall init: A,
+      (forall x, inv x -> f x = g x) ->
+      inv (init) ->
+      (forall x, inv x -> inv (g x)) ->
+      eq (coiterate f init) (coiterate g init).
+  Admitted.
+
+  Lemma map_eqn {A B} (f: A -> B) (s: Streams.Stream A) :
+    Streams.map f s =
+    f (Streams.hd s) ::: Streams.map f (Streams.tl s).
+  Proof.
+    rewrite (Streams.unfold_Stream (Streams.map f s)) at 1; reflexivity.
+  Qed.
+
+  Lemma Str_nth_0 {A} (hd: A) tl:
+    Streams.Str_nth 0 (hd ::: tl) = hd.
+  Proof. reflexivity. Qed.
+
+  Lemma Str_nth_S {A} (hd: A) tl n:
+    Streams.Str_nth (S n) (hd ::: tl) = Streams.Str_nth n tl.
+  Proof. reflexivity. Qed.
+End Streams.
+
+Arguments wp_action {pos_t var_t fn_name_t} {reg_t ext_fn_t} {R Sigma} {REnv} r sigma
+          {sig tau} _ !_ _ /.
+
+Arguments interp_cycle_cps {pos_t var_t fn_name_t rule_name_t reg_t ext_fn_t}%type_scope {R Sigma}%function_scope {REnv} r (sigma rules)%function_scope !s / {A}%type_scope k : assert.
+Arguments interp_scheduler_cps {pos_t var_t fn_name_t rule_name_t reg_t ext_fn_t}%type_scope {R Sigma}%function_scope {REnv} r (sigma rules)%function_scope !s / {A}%type_scope k : assert.
+Arguments interp_rule_cps {pos_t var_t fn_name_t reg_t ext_fn_t}%type_scope {R Sigma}%function_scope {REnv} r sigma%function_scope !rl / {A}%type_scope k log : assert.
+
+Arguments wp_scheduler {pos_t var_t fn_name_t rule_name_t reg_t ext_fn_t}%type_scope {R Sigma}%function_scope {REnv} r (sigma rules)%function_scope !s / post : assert.
+
+Arguments interp_cycle: simpl never.
+Arguments id _ _ / : assert.
+
+Declare Custom Entry context_mapping.
+
+Notation "x  ->  y" :=
+  (CtxCons x y CtxEmpty)
+    (in custom context_mapping at level 80,
+        x constr at level 0, y constr at level 80,
+        no associativity).
+
+Notation "x  ->  y ;  z" :=
+  (CtxCons x y z)
+    (in custom context_mapping at level 80,
+        x constr at level 0, y constr at level 80,
+        z custom context_mapping at level 80,
+        right associativity).
+
+Notation "#{  x  }#" := (x) (at level 0, x custom context_mapping at level 200) : context.
+Arguments env_t: simpl never.
+Arguments vect: simpl never.
+
+Arguments wp_cycle {pos_t var_t fn_name_t rule_name_t reg_t ext_fn_t}%type_scope {R Sigma}%function_scope {REnv} r (sigma rules)%function_scope !s / post : assert.
+
+Notation "env .[ idx ]" := (getenv ContextEnv env idx) (at level 1, format "env .[ idx ]").
+(* FIXME remove these notations *)
+Notation "0b0" := {| vhd := false; vtl := _vect_nil |}.
+Notation "0b1" := {| vhd := true; vtl := _vect_nil |}.
+
+Arguments may_read /.
+Arguments may_write /.
+Arguments logentry_app {T}%type_scope !l1 !l2 /: assert.
+
+Opaque interp_cycle.
+
+Section Correctness.
   Context {REnv: Env reg_t}.
+  Context (sigma: forall f, Sig_denote (Sigma f)).
 
   Definition rls :=
     Eval cbv in rules.
 
   Instance FiniteType_reg_t : FiniteType reg_t := _.
 
-  Lemma beq_dec_refl {A} {EQ: EqDec A}:
-    forall a, beq_dec a a = true.
-  Proof.
-    intros.
-    unfold beq_dec.
-    rewrite eq_dec_refl; reflexivity.
-  Qed.
+  Section Experiments.
+    Context (r: ContextEnv.(env_t) R).
 
-  Context (r: ContextEnv.(env_t) R).
-  Context (sigma: forall f, Sig_denote (Sigma f)).
-
-  Arguments wp_action {pos_t var_t fn_name_t} {reg_t ext_fn_t} {R Sigma} {REnv} r sigma
-            {sig tau} _ !_ _ /.
-
-  Arguments interp_cycle_cps {pos_t var_t fn_name_t rule_name_t reg_t ext_fn_t}%type_scope {R Sigma}%function_scope {REnv} r (sigma rules)%function_scope !s / {A}%type_scope k : assert.
-  Arguments interp_scheduler_cps {pos_t var_t fn_name_t rule_name_t reg_t ext_fn_t}%type_scope {R Sigma}%function_scope {REnv} r (sigma rules)%function_scope !s / {A}%type_scope k : assert.
-  Arguments interp_rule_cps {pos_t var_t fn_name_t reg_t ext_fn_t}%type_scope {R Sigma}%function_scope {REnv} r sigma%function_scope !rl / {A}%type_scope k log : assert.
-
-  Arguments wp_scheduler {pos_t var_t fn_name_t rule_name_t reg_t ext_fn_t}%type_scope {R Sigma}%function_scope {REnv} r (sigma rules)%function_scope !s / post : assert.
-
-  Arguments interp_cycle: simpl never.
-  Arguments id _ _ / : assert.
-
-  Declare Custom Entry context_mapping.
-
-  Notation "x  ->  y" :=
-    (CtxCons x y CtxEmpty)
-      (in custom context_mapping at level 80,
-          x constr at level 0, y constr at level 80,
-          no associativity).
-
-  Notation "x  ->  y ;  z" :=
-    (CtxCons x y z)
-      (in custom context_mapping at level 80,
-          x constr at level 0, y constr at level 80,
-          z custom context_mapping at level 80,
-          right associativity).
-
-  Notation "#{  x  }#" := (x) (at level 0, x custom context_mapping at level 200) : context.
-  Arguments env_t: simpl never.
-  Arguments vect: simpl never.
-
-  Arguments wp_cycle {pos_t var_t fn_name_t rule_name_t reg_t ext_fn_t}%type_scope {R Sigma}%function_scope {REnv} r (sigma rules)%function_scope !s / post : assert.
-
-  Notation "env .[ idx ]" := (getenv ContextEnv env idx) (at level 1, format "env .[ idx ]").
-  (* FIXME remove these notations *)
-  Notation "0b0" := {| vhd := false; vtl := _vect_nil |}.
-  Notation "0b1" := {| vhd := true; vtl := _vect_nil |}.
-
-  Arguments may_read /.
-  Arguments may_write /.
-  Arguments logentry_app {T}%type_scope !l1 !l2 /: assert.
-
-  Lemma cycle_correct :
-    forall (init: ContextEnv.(env_t) R),
-    exists l', Logs.commit_update init (TypedSemantics.interp_scheduler init sigma rls pipeline) = l'.
-  Proof.
-    intros; unfold pipeline.
-    (* Time unfold TypedSemantics.interp_scheduler, *)
-    (* TypedSemantics.interp_scheduler', *)
-    (* TypedSemantics.interp_rule; simpl. (* 11s *) *)
-  Abort.
-
-  Lemma cycle_correct :
-    forall (init: ContextEnv.(env_t) R),
-    exists l', CompactLogs.commit_update init (CompactSemantics.interp_scheduler init sigma rls pipeline) = l'.
-  Proof.
-    intros; unfold pipeline.
-    (* Time unfold CompactSemantics.interp_scheduler, CompactSemantics.interp_scheduler', CompactSemantics.interp_rule; simpl. (* 17s *) *)
-  Abort.
-
-  Lemma cycle_correct :
-    forall (init: ContextEnv.(env_t) R),
-    exists l', WP.interp_cycle init sigma rls pipeline = l'.
-  Proof.
-    intros; unfold pipeline.
-    apply wp_cycle_correct.
-    Time simpl. (* 0.7s *)
-
-    destruct (Bits.single init.[queue_empty]); simpl.
-    - (* Initialization: nothing in the queue yet *)
-      eexists; reflexivity.
-    - (* Steady state: queue remains full *)
-      eexists; reflexivity.
-  Qed.
-
-  Lemma scheduler_correct :
-    exists l', interp_scheduler r sigma rls pipeline = l'.
-  Proof.
-    unfold pipeline.
-    (* unfold interp_scheduler, interp_scheduler', interp_rule; simpl. *)
-    (* rewrite <- interp_scheduler_cps_correct; simpl. *)
-    apply wp_scheduler_correct.
-    Time simpl.
-    destruct (Bits.single (getenv ContextEnv r queue_empty)); simpl.
-    all: eexists; reflexivity.
-  Qed.
-
-  Require Lists.Streams.
-  Declare Scope stream_scope.
-  Infix ":::" := Streams.Cons (at level 60, right associativity) : stream_scope.
-
-  Section Traces.
-    Open Scope stream_scope.
-
-    CoFixpoint iterate {A} (f: A -> A) (init: A) :=
-      init ::: iterate f (f init).
-
-    Lemma iterate_eqn {A} (f: A -> A) (init: A) :
-      iterate f init =
-      init ::: iterate f (f init).
+    Lemma cycle_correct :
+      forall (init: ContextEnv.(env_t) R),
+      exists l', Logs.commit_update init (TypedSemantics.interp_scheduler init sigma rls pipeline) = l'.
     Proof.
-      rewrite (Streams.unfold_Stream (iterate f init)) at 1; reflexivity.
-    Qed.
-
-    Lemma map_eqn {A B} (f: A -> B) (s: Streams.Stream A) :
-      Streams.map f s =
-      f (Streams.hd s) ::: Streams.map f (Streams.tl s).
-    Proof.
-      rewrite (Streams.unfold_Stream (Streams.map f s)) at 1; reflexivity.
-    Qed.
-
-    (* Spec: The stream of inputs *)
-    Definition spec_inputs :=
-      iterate (sigma NextInput) r.[input_buffer].
-
-    (* Spec: The stream of outputs *)
-    Definition spec_outputs :=
-      let composed x := sigma G (sigma F x) in
-      r.[output_buffer] ::: r.[output_buffer] ::: Streams.map composed spec_inputs.
-
-    Definition states_trace :=
-      iterate (fun r: env_t _ R => interp_cycle r sigma rls pipeline) r.
-
-    Definition observable_trace :=
-      Streams.map (fun r: env_t _ R => r.[output_buffer]) states_trace.
-
-    Import Streams.
-
-    Ltac autorew :=
-      (* The variant below isn't enough, because primitive projections are weird *)
-      (* | [ H: ?a = _ |- _ ] => *)
-      (*   match goal with (* Merging the two matches together results in a 20x slowdown *) *)
-      (*   | [  |- context[a] ] => rewrite !H *)
-      (*   end *)
-      repeat match goal with
-             | [ H: ?a = ?a' |- context[match ?b with _ => _ end] ] =>
-               unify a b; replace b with a' by assumption
-             end.               (* FIXME doesn't work here *)
-
-    Lemma interp_pipeline_eqn :
-      forall r: ContextEnv.(env_t) R,
-        r.[queue_empty] = Ob~0 ->
-        interp_cycle r sigma rls pipeline =
-        #{ queue_data -> sigma F (r.[input_buffer]);
-           output_buffer -> sigma G r.[queue_data];
-           input_buffer -> sigma NextInput r.[input_buffer];
-           queue_empty -> Ob~0 }#.
-    Proof.
-      clear r; intros r H0.
-      apply wp_cycle_correct.
-      simpl.
-      rewrite H0; reflexivity.
-    Qed.
-
-    Lemma interp_pipeline_eqn2 :
-      forall r: ContextEnv.(env_t) R,
-        r.[queue_empty] = Ob~0 ->
-        interp_cycle (interp_cycle r sigma rls pipeline) sigma rls pipeline =
-        #{ queue_data -> sigma F (sigma NextInput r.[input_buffer]);
-           output_buffer -> sigma G (sigma F r.[input_buffer]);
-           input_buffer -> sigma NextInput (sigma NextInput r.[input_buffer]);
-           queue_empty -> Ob~0 }#.
-    Proof.
-      clear r; intros r H0.
-      Opaque interp_cycle.
-      rewrite (interp_pipeline_eqn r) by assumption; simpl.
-      rewrite interp_pipeline_eqn by reflexivity; simpl.
-      reflexivity.
-    Qed.
-
-    Theorem correct_pipeline:
-      r.[queue_empty] = Ob~1 ->
-      Streams.EqSt observable_trace spec_outputs.
-    Proof.
-      intros Hqueue_empty.
-      unfold observable_trace, spec_outputs, states_trace.
-      rewrite iterate_eqn.
-      rewrite interp_cycle_cps_correct_rev.
-      simpl.
-      rewrite Hqueue_empty.
-      simpl.
-      rewrite iterate_eqn.
-      rewrite interp_cycle_cps_correct_rev.
-      simpl.
-      rewrite map_eqn; simpl.
-      rewrite map_eqn; simpl.
-      constructor; [reflexivity | simpl tl].
-      constructor; [reflexivity | simpl tl].
+      intros; unfold pipeline.
+      (* Time unfold TypedSemantics.interp_scheduler, *)
+      (* TypedSemantics.interp_scheduler', *)
+      (* TypedSemantics.interp_rule; simpl. (* 11s *) *)
     Abort.
 
+    Lemma cycle_correct :
+      forall (init: ContextEnv.(env_t) R),
+      exists l', CompactLogs.commit_update init (CompactSemantics.interp_scheduler init sigma rls pipeline) = l'.
+    Proof.
+      intros; unfold pipeline.
+      (* Time unfold CompactSemantics.interp_scheduler, CompactSemantics.interp_scheduler', CompactSemantics.interp_rule; simpl. (* 17s *) *)
+    Abort.
+
+    Lemma cycle_correct :
+      forall (init: ContextEnv.(env_t) R),
+      exists l', WP.interp_cycle init sigma rls pipeline = l'.
+    Proof.
+      intros; unfold pipeline.
+      apply wp_cycle_correct.
+      Time simpl. (* 0.7s *)
+
+      destruct (Bits.single init.[queue_empty]); simpl.
+      - (* Initialization: nothing in the queue yet *)
+        eexists; reflexivity.
+      - (* Steady state: queue remains full *)
+        eexists; reflexivity.
+    Qed.
+
+    Lemma scheduler_correct :
+      exists l', interp_scheduler r sigma rls pipeline = l'.
+    Proof.
+      unfold pipeline.
+      (* unfold interp_scheduler, interp_scheduler', interp_rule; simpl. *)
+      (* rewrite <- interp_scheduler_cps_correct; simpl. *)
+      apply wp_scheduler_correct.
+      Time simpl.
+      destruct (Bits.single (getenv ContextEnv r queue_empty)); simpl.
+      all: eexists; reflexivity.
+    Qed.
+
+    Lemma scheduler_correct' :
+      (interp_scheduler r sigma rls pipeline).[input_buffer].(lwrite1) = None.
+    Proof.
+      unfold pipeline.
+      (* unfold interp_scheduler, interp_scheduler', interp_rule; simpl. *)
+      (* rewrite <- interp_scheduler_cps_correct; simpl. *)
+      apply wp_scheduler_correct.
+      Time simpl.
+      destruct (Bits.single (getenv ContextEnv r queue_empty)); simpl.
+      all: eexists; reflexivity.
+    Qed.
+
     Lemma doG_correct :
-      Bits.single (ContextEnv.(getenv) r queue_empty) = false ->
-      (* ContextEnv.(getenv) r queue_data = (sigma F) (ContextEnv.(getenv) r output_buffer) -> *)
+      Bits.single (r.[queue_empty]) = false ->
       exists l,
         interp_rule r sigma log_empty (rls doG) = Some l /\
         l.[queue_empty].(lwrite0) = Some Ob~1.
     (* FIXME: which style is better; exists or match? *)
     (* match interp_rule r sigma log_empty (rls doG) with *)
     (* | Some l => *)
-    (*   ContextEnv.(getenv) l queue_empty = [LE LogWrite P0 Ob~1; LE LogRead P0 tt] *)
+    (*   l.[queue_empty] = [LE LogWrite P0 Ob~1; LE LogRead P0 tt] *)
     (* | None => False *)
     (* end. *)
     Proof.
@@ -306,11 +338,22 @@ Section correct.
 
     Arguments env_t : simpl never.
 
+    Ltac autorew :=
+      (* The variant below isn't enough, because primitive projections are weird *)
+      (* | [ H: ?a = _ |- _ ] => *)
+      (*   match goal with (* Merging the two matches together results in a 20x slowdown *) *)
+      (*   | [  |- context[a] ] => rewrite !H *)
+      (*   end *)
+      repeat match goal with
+             | [ H: ?a = ?a' |- context[match ?b with _ => _ end] ] =>
+               unify a b; replace b with a' by assumption
+             end.               (* FIXME doesn't work here *)
+
     Lemma doF_correct :
       forall l,
-        let l_input_buffer := ContextEnv.(getenv) l input_buffer in
-        let l_queue_empty := ContextEnv.(getenv) l queue_empty in
-        let l_queue_data := ContextEnv.(getenv) l queue_data in
+        let l_input_buffer := l.[input_buffer] in
+        let l_queue_empty := l.[queue_empty] in
+        let l_queue_data := l.[queue_data] in
         l_input_buffer.(lwrite0) = None ->
         l_input_buffer.(lwrite1) = None ->
         l_input_buffer.(lread1) = false ->
@@ -319,7 +362,7 @@ Section correct.
         l_queue_data.(lwrite1) = None ->
         l_queue_empty.(lwrite1) = None ->
         l_queue_empty.(lwrite0) = Some Ob~1 ->
-        (* ContextEnv.(getenv) r queue_data = (sigma F) (ContextEnv.(getenv) r output_buffer) -> *)
+        (* r.[queue_data] = (sigma F) (r.[output_buffer]) -> *)
         exists l',
           interp_rule r sigma l (rls doF) = Some l'.
     Proof.
@@ -331,9 +374,112 @@ Section correct.
       Time simpl.
       Time autorew.
       simpl.
-      eexists; split; reflexivity.
+      eexists; reflexivity.
     Qed.
 
+    (* Compact encoding of preconditions *)
+    Lemma doF_correct' :
+      forall qd0 ob qe0 qe1 ib0,
+        let l :=
+            #{ queue_data -> {| lread0 := qd0; lread1 := false; lwrite0 := None; lwrite1 := None |};
+               output_buffer -> ob;
+               input_buffer -> {| lread0 := ib0; lread1 := false; lwrite0 := None; lwrite1 := None |};
+               queue_empty -> {| lread0 := qe0; lread1 := qe1; lwrite0 := Some Ob~1; lwrite1 := None |} }# in
+        exists l', interp_rule r sigma l (rls doF) = Some l'.
+    Proof.
+      intros.
+      unfold interp_rule.
+      apply (wp_action_correct (rule_name_t := rule_name_t)).
+      Time simpl.
+      (* Nothing to rewrite! *)
+      eexists; reflexivity.
+    Qed.
+  End Experiments.
+
+  Section Spec.
+    Context (r: ContextEnv.(env_t) R).
+
+    (* The stream of inputs consumed by the spec *)
+    Definition spec_inputs :=
+      coiterate (sigma NextInput) r.[input_buffer].
+
+    (* The expected stream of observable values *)
+    Definition spec_observations :=
+      let composed x := sigma G (sigma F x) in
+      r.[output_buffer] ::: r.[output_buffer] ::: Streams.map composed spec_inputs.
+
+    (* The actual stream of states produced by the implementation *)
+    Definition impl_trace :=
+      coiterate (fun r: env_t _ R => interp_cycle r sigma rls pipeline) r.
+
+    (* The actual stream of observations produced by the implementation *)
+    Definition impl_observations :=
+      Streams.map (fun r: env_t _ R => r.[output_buffer]) impl_trace.
+  End Spec.
+
+  Section Proofs.
+    Definition cycle (r: ContextEnv.(env_t) R) :=
+      interp_cycle r sigma rls pipeline.
+
+    Definition phi2
+               (r: ContextEnv.(env_t) R)
+      : ContextEnv.(env_t) R :=
+      #{ queue_data -> sigma F (sigma NextInput r.[input_buffer]);
+         output_buffer -> sigma G (sigma F r.[input_buffer]);
+         input_buffer -> sigma NextInput (sigma NextInput r.[input_buffer]);
+         queue_empty -> Ob~0 }#.
+
+    Lemma phi2_correct :
+      forall r, cycle (cycle r) = phi2 r.
+    Proof.
+      intros r; unfold cycle.
+      rewrite (interp_cycle_cps_correct_rev r); simpl.
+      destruct (Bits.single r.[queue_empty]); simpl.
+      all: rewrite interp_cycle_cps_correct_rev; simpl;
+        reflexivity.
+    Qed.
+
+    Definition phi_iterated n
+               (r: ContextEnv.(env_t) R)
+      : ContextEnv.(env_t) R :=
+      #{ queue_data -> sigma F (iterate (S n) (sigma NextInput) r.[input_buffer]);
+         output_buffer -> sigma G (sigma F (iterate n (sigma NextInput) r.[input_buffer]));
+         input_buffer -> iterate (S (S n)) (sigma NextInput) r.[input_buffer];
+         queue_empty -> Ob~0 }#.
+
+    Lemma phi_iterated_correct :
+      forall r n,
+        iterate (S (S n)) cycle r =
+        phi_iterated n r.
+    Proof.
+      intros r n.
+      rewrite !iterate_S_acc, phi2_correct.
+      revert n; apply Div2.ind_0_1_SS; simpl.
+      - reflexivity.
+      - unfold cycle; rewrite interp_cycle_cps_correct_rev; reflexivity.
+      - intros n IH; simpl in IH; rewrite IH; reflexivity.
+    Qed.
+
+    Theorem correct_pipeline:
+      forall r,
+        r.[queue_empty] = Ob~1 ->
+        Streams.EqSt (impl_observations r) (spec_observations r).
+    Proof.
+      intros r Hqueue_empty.
+      unfold impl_observations, spec_observations, impl_trace.
+
+      apply Streams.ntheq_eqst; intros [ | [ | n ] ]; simpl;
+        unfold spec_inputs;
+        rewrite ?Str_nth_0, ?Str_nth_S, ?Streams.Str_nth_map, ?Str_nth_coiterate.
+      - reflexivity.
+      - simpl.
+        rewrite interp_cycle_cps_correct_rev; simpl.
+        rewrite Hqueue_empty; reflexivity.
+      - rewrite phi_iterated_correct.
+        reflexivity.
+    Qed.
+  End Proofs.
+End Correctness.
 
 Definition external (r: rule_name_t) := false.
 
@@ -393,10 +539,3 @@ Definition package :=
 
 Definition prog := Interop.Backends.register package.
 Extraction "pipeline.ml" prog.
-
-
-  (* FIXME: is it a cbn bug that adding exclamation points below prevents reduction?*)
-  (* Probably due to implicits *)
-  (* Arguments may_read _ _ _ /. *)
-  (* Arguments may_write _ _ _ /. *)
-  (* cbn. *)
